Give up on well-scoped nbe

eval.v
@@ -15,6 +15,27 @@ with DomainNe (n : nat) : Type :=
 | DN_var (i : fin n) : DomainNe n
 | DN_App (d : DomainNe n) (e : Domain n) : DomainNe n.
 
+Definition embed {n} : fin n -> fin (S n).
+  elim : n => [//|/= n embed].
+  case => [m | ].
+  - exact (Some (embed m)).
+  - exact None.
+Defined.
+
+Definition max_fin {n} : fin (S n).
+  elim : n => [//|n max_fin].
+  - exact None.
+  - exact (Some max_fin).
+Defined.
+
+(* Need the inv operation to define read back  *)
+Definition inv {n} (m : fin n) : fin n.
+  elim : n m => /= [// | n inv].
+  case => [m|].
+  - exact (embed (inv m)).
+  - exact max_fin.
+Defined.
+
 Fixpoint ren_dom {n m} (ξ : fin n -> fin m) (a : Domain n) : Domain m :=
   match a with
   | D_Clos A a ρ => D_Clos A a (ρ >> ren_dom ξ)
@@ -45,61 +66,44 @@ with D_Eval {n} : forall {m}, Env m n -> tm m -> Domain n -> Prop :=
   D_Ap d0 d1 d2 ->
   D_Eval ρ (App a b) d2.
 
-Definition embed {n} : fin n -> fin (S n).
-  elim : n => [//|/= n embed].
-  case => [m | ].
-  - exact (Some (embed m)).
-  - exact None.
-Defined.
-
-Definition max_fin {n} : fin (S n).
-  elim : n => [//|n max_fin].
-  - exact None.
-  - exact (Some max_fin).
-Defined.
-
-(* Need the inv operation to define read back  *)
-Definition inv {n} (m : fin n) : fin n.
-  elim : n m => /= [// | n inv].
-  case => [m|].
-  - exact (embed (inv m)).
-  - exact max_fin.
-Defined.
+Scheme D_Ap_ind' := Induction for D_Ap Sort Prop
+   with D_Eval_ind' := Induction for D_Eval Sort Prop.
+Combined Scheme eval_mutual from D_Eval_ind', D_Ap_ind'.
 
 (* Need to show that inv is idempotent for the correctness proof  *)
-Lemma inv_embed_commute {n} (m : fin n) : Some (inv m) = inv (embed m).
-Proof.
-  elim : n m => [//| n ih m].
-  simpl in m.
-  case : m.
-  - hauto lq:on.
-  - reflexivity.
-Qed.
+(* Lemma inv_embed_commute {n} (m : fin n) : Some (inv m) = inv (embed m). *)
+(* Proof. *)
+(*   elim : n m => [//| n ih m]. *)
+(*   simpl in m. *)
+(*   case : m. *)
+(*   - hauto lq:on. *)
+(*   - reflexivity. *)
+(* Qed. *)
 
-Lemma inv_max_zero n : inv (@max_fin n) = None.
-Proof.
-  elim : n; hauto lq:on.
-Qed.
+(* Lemma inv_max_zero n : inv (@max_fin n) = None. *)
+(* Proof. *)
+(*   elim : n; hauto lq:on. *)
+(* Qed. *)
 
-Lemma inv_idempotent {n} (m : fin n) : inv (inv m) = m.
-Proof.
-  elim : n m => [// | n ihm m].
-  simpl in m.
-  case : m => [a|].
-  - hauto lq:on use:inv_embed_commute.
-  - sfirstorder use:inv_max_zero.
-Qed.
+(* Lemma inv_idempotent {n} (m : fin n) : inv (inv m) = m. *)
+(* Proof. *)
+(*   elim : n m => [// | n ihm m]. *)
+(*   simpl in m. *)
+(*   case : m => [a|]. *)
+(*   - hauto lq:on use:inv_embed_commute. *)
+(*   - sfirstorder use:inv_max_zero. *)
+(* Qed. *)
 
 Inductive Readback {n} : Domain n -> tm n -> Prop :=
 | R_Clos m (ρ : Env m n) (a : tm (S m)) d A b:
-  D_Eval (D_Ne (DN_var max_fin) .: (ρ >> ren_dom embed)) a d ->
+  D_Eval (D_Ne (DN_var var_zero) .: (ρ >> ren_dom shift)) a d ->
   @Readback (S n) d b ->
   Readback (D_Clos A a ρ : Domain n) (Lam A b : tm n)
 | R_Ne e a :
   ReadbackNe e a ->
   Readback (D_Ne e) a
 with ReadbackNe {n} : DomainNe n -> tm n -> Prop :=
-| R_Var i : ReadbackNe (DN_var i) (var_tm (inv i))
+| R_Var i : ReadbackNe (DN_var i) (var_tm i)
 | R_App e d a b :
   ReadbackNe e a ->
   Readback d b ->
@@ -112,41 +116,137 @@ with nf {n} : tm n -> Prop :=
 | nf_ne e : ne e -> nf e
 | nf_abs A a : nf (Lam A a).
 
-Definition TopSpace {n} (d : Domain n) :=
-  exists v, nf v /\ Readback d v.
+Scheme ne_ind' := Induction for ne Sort Prop
+   with nf_ind' := Induction for nf Sort Prop.
+Combined Scheme ne_mutual from ne_ind', nf_ind'.
 
-Definition BotSpaceNe {n} (e : DomainNe n) :=
-  exists u, ne u /\ ReadbackNe e u.
+Scheme Readback_ind' := Induction for Readback Sort Prop
+    with ReadbackNe_ind' := Induction for ReadbackNe Sort Prop.
+Combined Scheme Readback_mutual from Readback_ind', ReadbackNe_ind'.
 
-Definition BotSpace {n} (d : Domain n) :=
+Definition TopSpace n (d : Domain n) :=
+  exists v, nf v /\ @Readback n d v.
+
+Definition BotSpaceNe n (e : DomainNe n) :=
+  exists u, ne u /\ @ReadbackNe n e u.
+
+Definition BotSpace n (d : Domain n) :=
   match d with
-  | D_Ne e => BotSpaceNe e
+  | D_Ne e => @BotSpaceNe n e
   | _ => False
   end.
 
-Definition SemFun {n} (A : Domain n -> Prop) (B : Domain n -> Prop) (b : Domain n) :=
-  forall a, A a -> exists d, B d /\ D_Ap b a d.
+Definition SemFun n (A : forall n, Domain n -> Prop) (B : forall n, Domain n -> Prop) (b : Domain n) :=
+  forall m (a : Domain m) (ξ : fin n -> fin m),
+    A m a ->
+    exists d, B m d /\ D_Ap (ren_dom ξ b) a d.
 
 #[export]Hint Unfold BotSpace TopSpace BotSpaceNe SemFun : core.
+
+Lemma renaming_ne_nf n :
+  (forall a : tm n, ne a -> forall m (ξ : fin n -> fin m), ne (ren_tm ξ a)) /\
+  (forall a : tm n, nf a -> forall m (ξ : fin n -> fin m), nf (ren_tm ξ a)).
+Proof.
+  apply ne_mutual; hauto lq:on ctrs:ne,nf.
+Qed.
+
+Lemma R_Clos' n m (ρ : Env m n) (a : tm (S m)) d A b b0:
+  b0 = (Lam A b : tm n) ->
+  D_Eval (D_Ne (DN_var var_zero) .: (ρ >> ren_dom shift)) a d ->
+  @Readback (S n) d b ->
+  Readback (D_Clos A a ρ : Domain n) b0.
+Proof.
+  move => *; subst.
+  sfirstorder use:R_Clos.
+Qed.
+
+(* Inductive D_Ap {n} : Domain n -> Domain n -> Domain n -> Prop := *)
+(* with D_Eval {n} : forall {m}, Env m n -> tm m -> Domain n -> Prop := *)
+
+Lemma renaming_eval_mutual n :
+  (forall {p} (ρ : Env p n) (a : tm p) (d : Domain n),
+      D_Eval ρ a d -> forall m (ξ : fin n -> fin m), D_Eval (ρ >> ren_dom ξ) a (ren_dom ξ d)) /\
+    (forall (d0 d1 d2 : Domain n), D_Ap d0 d1 d2 ->
+                              forall m (ξ : fin n -> fin m),
+                              D_Ap (ren_dom ξ d0) (ren_dom ξ d1) (ren_dom ξ d2)).
+Proof.
+  apply eval_mutual.
+  - sfirstorder.
+  - move => p a A ρ d0 d1 h0 ih0 m ξ.
+    simpl.
+    apply DAp_App.
+    move /(_ m ξ) in ih0.
+    by asimpl in ih0.
+  - sfirstorder.
+  - sfirstorder.
+  - hauto lq:on ctrs:D_Eval.
+Qed.
+
+Lemma renaming_eval n :
+  (forall {p} (ρ : Env p n) (a : tm p) (d : Domain n),
+      D_Eval ρ a d -> forall m (ξ : fin n -> fin m), D_Eval (ρ >> ren_dom ξ) a (ren_dom ξ d)).
+Proof. hauto l:on use:renaming_eval_mutual. Qed.
+
+Lemma renaming_eval_weaken :
+  forall {n p} (ρ : Env p n) (a : tm p) (d : Domain n),
+    D_Eval ρ a d -> D_Eval (ρ >> ren_dom shift) a (ren_dom shift d).
+Proof.
+  move=> n p ρ a d h0.
+  by apply renaming_eval.
+Qed.
+
+Lemma renaming_readback_mutual n :
+  (forall (d : Domain n) (u : tm n), Readback d u -> forall m (ξ : fin n -> fin m),
+        Readback (ren_dom ξ d) (ren_tm ξ u) ) /\
+  (forall (e : DomainNe n) (v : tm n), ReadbackNe e v -> forall m (ξ : fin n -> fin m),
+        ReadbackNe (ren_domNe ξ e) (ren_tm ξ v) ).
+Proof.
+  move : n.
+  apply Readback_mutual.
+  - move => n p ρ a d A b h0 h1 ih1 m ξ /=.
+    apply : R_Clos'; eauto.
+    asimpl in h0.
+    apply renaming_eval with (ξ := (var_zero .: ξ >> ↑)) in h0.
+    asimpl in h0.
+    simpl in h0.
+    (* need to come up with the necessary rewriting rules *)
+    admit.
+  - hauto lq:on ctrs:Readback.
+  - move => n i m ξ.
+    asimpl.
+    simpl.
+    sfirstorder.
+Admitted.
 
 Lemma cand_prop1 {n} (d : Domain n) : BotSpace d -> SemFun TopSpace BotSpace d.
 Proof.
   rewrite /SemFun.
-  move => h a ha.
+  move => h m a ξ ha.
   rewrite /BotSpace /TopSpace in h ha.
   case : d h => [// | d h].
   case : ha => v [hv0 hv1].
-  exists (D_Ne (DN_App d a)).
+  exists (D_Ne (DN_App (ren_domNe ξ d) a)).
   split.
   - rewrite /BotSpace.
     rewrite /BotSpaceNe in h *.
     case : h => u [hu0 hu1].
-    exists (App u v).
+    exists (App (ren_tm ξ u) v).
     split.
-    + hauto lq:on ctrs:ne.
-    + hauto lq:on ctrs:ReadbackNe.
+    + hauto l:on use:renaming_ne_nf.
+    + apply R_App; auto.
+      hauto l:on use:renaming_readback_mutual.
   - sfirstorder.
 Qed.
+
+Lemma cand_prop2 {n} (d : Domain n) : SemFun BotSpace TopSpace d -> TopSpace d.
+Proof.
+  move => h.
+  rewrite /SemFun in h.
+  move /(_ (S n) (D_Ne (DN_var var_zero)) shift ltac:(hauto l:on)) in h.
+  move : h; intros (d0 & h0 & h1).
+  rewrite /TopSpace.
+Admitted.
+
 
 Fixpoint Interp {n} (A : ty) (f : Domain n) : Prop :=
   match A with
